code/bignum/Hacl.Bignum64.fst
@@ -6,48 +6,50 @@ module BN = Hacl.Bignum
 module BM = Hacl.Bignum.Montgomery
 module BE = Hacl.Bignum.Exponentiation
 module BR = Hacl.Bignum.ModReduction
+module AM = Hacl.Bignum.AlmostMontgomery
 
 #set-options "--z3rlimit 50 --fuel 0 --ifuel 0"
+
+inline_for_extraction noextract
+let kam (len:BN.meta_len t_limbs) =
+  AM.mk_runtime_almost_mont #t_limbs len
 
 inline_for_extraction noextract
 let ke (len:BN.meta_len t_limbs) =
   BE.mk_runtime_exp #t_limbs len
 
 let add len a b res =
-  (ke len).BE.mont.BM.bn.BN.add a b res
+  (ke len).BE.bn.BN.add a b res
 
 let sub len a b res =
-  (ke len).BE.mont.BM.bn.BN.sub a b res
+  (ke len).BE.bn.BN.sub a b res
 
 let mul len a b res =
-  (ke len).BE.mont.BM.bn.BN.mul a b res
+  (ke len).BE.bn.BN.mul a b res
 
 let sqr len a res =
-  (ke len).BE.mont.BM.bn.BN.sqr a res
-
-let mod_precompr2 len n a r2 res =
-  BR.bn_mod_slow_precompr2 (ke len).BE.mont n a r2 res
+  (ke len).BE.bn.BN.sqr a res
 
 let mod len n a res =
-  BS.bn_mod_slow_safe (ke len).BE.mont (mod_precompr2 len) n a res
+  BS.mk_bn_mod_slow_safe (kam len) (BR.bn_mod_slow_precompr2 (kam len)) n a res
 
-let mod_exp_vartime_precompr2 len n a bBits b r2 res =
-  BE.bn_mod_exp_vartime_precompr2 (ke len) n a bBits b r2 res
+// let mod_exp_vartime_precompr2 len n a bBits b r2 res =
+//   BE.bn_mod_exp_vartime_precompr2 (ke len) n a bBits b r2 res
 
-let mod_exp_consttime_precompr2 len n a bBits b r2 res =
-  BE.bn_mod_exp_consttime_precompr2 (ke len) n a bBits b r2 res
+// let mod_exp_consttime_precompr2 len n a bBits b r2 res =
+//   BE.bn_mod_exp_consttime_precompr2 (ke len) n a bBits b r2 res
 
 let mod_exp_vartime len n a bBits b res =
-  BS.bn_mod_exp_vartime_safe (ke len) (mod_exp_vartime_precompr2 len) n a bBits b res
+  BS.mk_bn_mod_exp_safe (ke len) (ke len).BE.exp_vt n a bBits b res
 
 let mod_exp_consttime len n a bBits b res =
-  BS.bn_mod_exp_consttime_safe (ke len) (mod_exp_consttime_precompr2 len) n a bBits b res
+  BS.mk_bn_mod_exp_safe (ke len) (ke len).BE.exp_ct n a bBits b res
 
-let new_precompr2 len r n =
-  BS.new_bn_precomp_r2_mod_n (ke len).BE.mont r n
+// let new_precompr2 len r n =
+//   BS.new_bn_precomp_r2_mod_n (ke len).BE.mont r n
 
 let mod_inv_prime_vartime len n a res =
-  BS.bn_mod_inv_prime_vartime_safe (ke len) (mod_exp_vartime_precompr2 len) n a res
+  BS.mk_bn_mod_inv_prime_safe len (ke len).BE.exp_vt n a res
 
 let new_bn_from_bytes_be r len b =
   BS.new_bn_from_bytes_be r len b
