code/bignum/Hacl.Bignum32.fsti
@@ -35,14 +35,14 @@ Comment
 
   This functions returns the carry.
 
-  The arguments a, b and res are meant to be `len` limbs in size, i.e. uint32_t[len]"]
+  The arguments a, b and the outparam res are meant to be `len` limbs in size, i.e. uint32_t[len]"]
 val add: len:BN.meta_len t_limbs -> BN.bn_add_eq_len_st t_limbs len
 
 [@@ Comment "Write `a - b mod 2 ^ (32 * len)` in `res`.
 
   This functions returns the carry.
 
-  The arguments a, b and res are meant to be `len` limbs in size, i.e. uint32_t[len]"]
+  The arguments a, b and the outparam res are meant to be `len` limbs in size, i.e. uint32_t[len]"]
 val sub: len:BN.meta_len t_limbs -> BN.bn_sub_eq_len_st t_limbs len
 
 [@@ Comment "Write `a * b` in `res`.
@@ -57,83 +57,86 @@ val mul: len:BN.meta_len t_limbs -> a:lbignum t_limbs len -> BN.bn_karatsuba_mul
   The outparam res is meant to be `2*len` limbs in size, i.e. uint32_t[2*len]."]
 val sqr: len:BN.meta_len t_limbs -> a:lbignum t_limbs len -> BN.bn_karatsuba_sqr_st t_limbs len a
 
-[@@ Comment "Write `a mod n` in `res` if a < n * n.
+// [@@ Comment "Write `a mod n` in `res`.
 
-  The argument a is meant to be `2*len` limbs in size, i.e. uint32_t[2*len].
-  The argument n, r2 and the outparam res are meant to be `len` limbs in size, i.e. uint32_t[len].
-  The argument r2 is a precomputed constant 2 ^ (64 * len) mod n obtained through Hacl_Bignum32_new_precompr2.
+//   The argument a is meant to be `2*len` limbs in size, i.e. uint32_t[2*len].
+//   The argument n, r2 and the outparam res are meant to be `len` limbs in size, i.e. uint32_t[len].
+//   The argument r2 is a precomputed constant 2 ^ (128 * len) mod n obtained through Hacl_Bignum32_new_precompr2.
 
-  This function is *UNSAFE* and requires C clients to observe the precondition
-  of bn_mod_slow_precompr2_lemma in Hacl.Spec.Bignum.ModReduction.fst, which
-  amounts to:
-  • 1 < n
-  • n % 2 = 1
-  • a < n * n
+//   This function is *UNSAFE* and requires C clients to observe the precondition
+//   of bn_mod_slow_precompr2_lemma in Hacl.Spec.Bignum.ModReduction.fst, which
+//   amounts to:
+//   • 1 < n
+//   • n % 2 = 1
+//   • a < n * n
 
-  Owing to the absence of run-time checks, and factoring out the precomputation
-  r2, this function is notably faster than mod below."]
-val mod_precompr2: len:BN.meta_len t_limbs -> BR.bn_mod_slow_precompr2_st t_limbs len
+//   Owing to the absence of run-time checks, and factoring out the precomputation
+//   r2, this function is notably faster than mod below."]
+// val mod_precompr2: len:BN.meta_len t_limbs -> BR.bn_mod_slow_precompr2_st t_limbs len
 
-[@@ Comment "Write `a mod n` in `res` if a < n * n.
+[@@ Comment "Write `a mod n` in `res`.
 
   The argument a is meant to be `2*len` limbs in size, i.e. uint32_t[2*len].
   The argument n and the outparam res are meant to be `len` limbs in size, i.e. uint32_t[len].
 
-  The function returns false if any of the preconditions of mod_precompr2 above
-  are violated, true otherwise."]
+  The function returns false if any of the following preconditions are violated,
+  true otherwise.
+   • 1 < n
+   • n % 2 = 1 "]
 val mod: len:BN.meta_len t_limbs -> BS.bn_mod_slow_safe_st t_limbs len
 
-[@@ Comment "Write `a ^ b mod n` in `res`.
+// [@@ Comment "Write `a ^ b mod n` in `res`.
 
-  The arguments a, n, r2 and the outparam res are meant to be `len` limbs in size, i.e. uint32_t[len].
-  The argument r2 is a precomputed constant 2 ^ (64 * len) mod n obtained through Hacl_Bignum32_new_precompr2.
-  The argument b is a bignum of any size, and bBits is an upper bound on the
-  number of significant bits of b. A tighter bound results in faster execution
-  time. When in doubt, the number of bits for the bignum size is always a safe
-  default, e.g. if b is a 4096-bit bignum, bBits should be 4096.
+//   The arguments a, n, r2 and the outparam res are meant to be `len` limbs in size, i.e. uint32_t[len].
+//   The argument r2 is a precomputed constant 2 ^ (128 * len) mod n obtained through Hacl_Bignum32_new_precompr2.
+//   The argument b is a bignum of any size, and bBits is an upper bound on the
+//   number of significant bits of b. A tighter bound results in faster execution
+//   time. When in doubt, the number of bits for the bignum size is always a safe
+//   default, e.g. if b is a 4096-bit bignum, bBits should be 4096.
 
-  The function is *NOT* constant-time on the argument b. See the
-  mod_exp_consttime_* functions for constant-time variants.
+//   The function is *NOT* constant-time on the argument b. See the
+//   mod_exp_consttime_* functions for constant-time variants.
 
-  This function is *UNSAFE* and requires C clients to observe bn_mod_exp_pre
-  from Hacl.Spec.Bignum.Exponentiation.fsti, which amounts to:
-  • n % 2 = 1
-  • 1 < n
-  • 0 < b
-  • b < pow2 bBits
-  • a < n
+//   This function is *UNSAFE* and requires C clients to observe bn_mod_exp_pre
+//   from Hacl.Spec.Bignum.Exponentiation.fsti, which amounts to:
+//   • n % 2 = 1
+//   • 1 < n
+//   • 0 < b
+//   • b < pow2 bBits
+//   • a < n
 
-  Owing to the absence of run-time checks, and factoring out the precomputation
-  r2, this function is notably faster than mod_exp_vartime below."]
-val mod_exp_vartime_precompr2: len:BN.meta_len t_limbs -> BE.bn_mod_exp_precompr2_st t_limbs len
+//   Owing to the absence of run-time checks, and factoring out the precomputation
+//   r2, this function is notably faster than mod_exp_vartime below."]
+// val mod_exp_vartime_precompr2: len:BN.meta_len t_limbs -> BE.bn_mod_exp_precompr2_st t_limbs len
 
-[@@ Comment "Write `a ^ b mod n` in `res`.
+// [@@ Comment "Write `a ^ b mod n` in `res`.
 
-  The arguments a, n, r2 and the outparam res are meant to be `len` limbs in size, i.e. uint32_t[len].
-  The argument r2 is a precomputed constant 2 ^ (64 * len) mod n obtained through Hacl_Bignum32_new_precompr2.
-  The argument b is a bignum of any size, and bBits is an upper bound on the
-  number of significant bits of b. A tighter bound results in faster execution
-  time. When in doubt, the number of bits for the bignum size is always a safe
-  default, e.g. if b is a 4096-bit bignum, bBits should be 4096.
+//   The arguments a, n, r2 and the outparam res are meant to be `len` limbs in size, i.e. uint32_t[len].
+//   The argument r2 is a precomputed constant 2 ^ (128 * len) mod n obtained through Hacl_Bignum32_new_precompr2.
+//   The argument b is a bignum of any size, and bBits is an upper bound on the
+//   number of significant bits of b. A tighter bound results in faster execution
+//   time. When in doubt, the number of bits for the bignum size is always a safe
+//   default, e.g. if b is a 4096-bit bignum, bBits should be 4096.
 
-  This function is constant-time over its argument b, at the cost of a slower
-  execution time than mod_exp_vartime_precompr2.
+//   This function is constant-time over its argument b, at the cost of a slower
+//   execution time than mod_exp_vartime_precompr2.
 
-  This function is *UNSAFE* and requires C clients to observe bn_mod_exp_pre
-  from Hacl.Spec.Bignum.Exponentiation.fsti, which amounts to:
-  • n % 2 = 1
-  • 1 < n
-  • 0 < b
-  • b < pow2 bBits
-  • a < n
+//   This function is *UNSAFE* and requires C clients to observe bn_mod_exp_pre
+//   from Hacl.Spec.Bignum.Exponentiation.fsti, which amounts to:
+//   • n % 2 = 1
+//   • 1 < n
+//   • 0 < b
+//   • b < pow2 bBits
+//   • a < n
 
-  Owing to the absence of run-time checks, and factoring out the precomputation
-  r2, this function is notably faster than mod_exp_consttime below."]
-val mod_exp_consttime_precompr2: len:BN.meta_len t_limbs -> BE.bn_mod_exp_precompr2_st t_limbs len
+//   Owing to the absence of run-time checks, and factoring out the precomputation
+//   r2, this function is notably faster than mod_exp_consttime below."]
+// val mod_exp_consttime_precompr2: len:BN.meta_len t_limbs -> BE.bn_mod_exp_precompr2_st t_limbs len
 
 [@@ Comment "Write `a ^ b mod n` in `res`.
 
   The arguments a, n and the outparam res are meant to be `len` limbs in size, i.e. uint32_t[len].
+
   The argument b is a bignum of any size, and bBits is an upper bound on the
   number of significant bits of b. A tighter bound results in faster execution
   time. When in doubt, the number of bits for the bignum size is always a safe
@@ -142,13 +145,19 @@ val mod_exp_consttime_precompr2: len:BN.meta_len t_limbs -> BE.bn_mod_exp_precom
   The function is *NOT* constant-time on the argument b. See the
   mod_exp_consttime_* functions for constant-time variants.
 
-  The function returns false if any of the preconditions of mod_exp_precompr2 are
-  violated, true otherwise."]
+  The function returns false if any of the following preconditions are violated,
+  true otherwise.
+   • n % 2 = 1
+   • 1 < n
+   • 0 < b
+   • b < pow2 bBits
+   • a < n "]
 val mod_exp_vartime: len:BN.meta_len t_limbs -> BS.bn_mod_exp_safe_st t_limbs len
 
 [@@ Comment "Write `a ^ b mod n` in `res`.
 
   The arguments a, n and the outparam res are meant to be `len` limbs in size, i.e. uint32_t[len].
+
   The argument b is a bignum of any size, and bBits is an upper bound on the
   number of significant bits of b. A tighter bound results in faster execution
   time. When in doubt, the number of bits for the bignum size is always a safe
@@ -157,30 +166,36 @@ val mod_exp_vartime: len:BN.meta_len t_limbs -> BS.bn_mod_exp_safe_st t_limbs le
   This function is constant-time over its argument b, at the cost of a slower
   execution time than mod_exp_vartime.
 
-  The function returns false if any of the preconditions of
-  mod_exp_consttime_precompr2 are violated, true otherwise."]
+  The function returns false if any of the following preconditions are violated,
+  true otherwise.
+   • n % 2 = 1
+   • 1 < n
+   • 0 < b
+   • b < pow2 bBits
+   • a < n "]
 val mod_exp_consttime: len:BN.meta_len t_limbs -> BS.bn_mod_exp_safe_st t_limbs len
 
-[@@ Comment "Compute `2 ^ (64 * len) mod n`.
+// [@@ Comment "Compute `2 ^ (128 * len) mod n`.
 
-  The argument n points to `len` limbs of valid memory.
-  The function returns a heap-allocated bignum of size `len`, or NULL if:
-  • the allocation failed, or
-  • n % 2 = 1 && 1 < n does not hold
+//   The argument n points to `len` limbs of valid memory.
+//   The function returns a heap-allocated bignum of size `len`, or NULL if:
+//   • the allocation failed, or
+//   • n % 2 = 1 && 1 < n does not hold
 
-  If the return value is non-null, clients must eventually call free(3) on it to
-  avoid memory leaks."]
-val new_precompr2: len:BN.meta_len t_limbs -> BS.new_bn_precomp_r2_mod_n_st t_limbs len
+//   If the return value is non-null, clients must eventually call free(3) on it to
+//   avoid memory leaks."]
+// val new_precompr2: len:BN.meta_len t_limbs -> BS.new_bn_precomp_r2_mod_n_st t_limbs len
 
 [@@ Comment "Write `a ^ (-1) mod n` in `res`.
 
   The arguments a, n and the outparam res are meant to be `len` limbs in size, i.e. uint32_t[len].
 
-  This function is *UNSAFE* and requires C clients to observe bn_mod_inv_prime_pre
-  from Hacl.Spec.Bignum.ModInv.fst, which amounts to:
+  Before calling this function, the caller will need to ensure that the following
+  preconditions are observed.
   • n is a prime
 
-  The function returns false if any of the following preconditions are violated, true otherwise.
+  The function returns false if any of the following preconditions are violated,
+  true otherwise.
   • n % 2 = 1
   • 1 < n
   • 0 < a
@@ -216,13 +231,13 @@ val new_bn_from_bytes_le: BS.new_bn_from_bytes_le_st t_limbs
 
 [@@ Comment "Serialize a bignum into big-endian memory.
 
-  The argument b points to a bignum of `32 * len` size.
+  The argument b points to a bignum of ⌈len / 32⌉ size.
   The outparam res points to `len` bytes of valid memory."]
 val bn_to_bytes_be: len:_ -> Hacl.Bignum.Convert.bn_to_bytes_be_st t_limbs len
 
 [@@ Comment "Serialize a bignum into little-endian memory.
 
-  The argument b points to a bignum of `32 * len` size.
+  The argument b points to a bignum of ⌈len / 32⌉ size.
   The outparam res points to `len` bytes of valid memory."]
 val bn_to_bytes_le: len:_ -> Hacl.Bignum.Convert.bn_to_bytes_le_st t_limbs len
 
@@ -231,5 +246,6 @@ val bn_to_bytes_le: len:_ -> Hacl.Bignum.Convert.bn_to_bytes_le_st t_limbs len
 /* Comparisons */
 /***************/\n";
 Comment
-"Returns 2 ^ 32 - 1 if and only if argument a is strictly less than the argument b, otherwise returns 0."]
+"Returns 2 ^ 32 - 1 if and only if the argument a is strictly less than the argument b,
+ otherwise returns 0."]
 val lt_mask: len:BN.meta_len t_limbs -> BN.bn_lt_mask_st t_limbs len
