code/bignum/Hacl.GenericField32.fsti
@@ -34,12 +34,20 @@ Comment "Check whether this library will work for a modulus `n`.
   • 1 < n "]
 val field_modulus_check: len:BN.meta_len t_limbs -> MA.bn_field_check_modulus_st t_limbs len
 
-[@@ Comment "Allocate and initialize a montgomery context.
+[@@ Comment "Heap-allocate and initialize a montgomery context.
 
-  The argument n is meant to be `len` limbs in size, i.e. uint32_t[len]."]
+  The argument n is meant to be `len` limbs in size, i.e. uint32_t[len].
+
+  The caller will need to call Hacl_GenericField32_field_free on the return value
+  to avoid memory leaks."]
 val field_init: len:BN.meta_len t_limbs -> MA.bn_field_init_st t_limbs len
 
-[@@ Comment "Return a size of the modulus `n` in limbs.
+[@@ Comment "Deallocate the memory previously allocated by Hacl_GenericField32_field_init.
+
+  The argument k is a montgomery context obtained through Hacl_GenericField32_field_init."]
+val field_free: MA.bn_field_free_st t_limbs
+
+[@@ Comment "Return the size of a modulus `n` in limbs.
 
   The argument k is a montgomery context obtained through Hacl_GenericField32_field_init."]
 val field_get_len: k:MA.bn_mont_ctx_u32 -> MA.bn_field_get_len_st k
@@ -48,7 +56,7 @@ val field_get_len: k:MA.bn_mont_ctx_u32 -> MA.bn_field_get_len_st k
 
   Write `a * R mod n` in `aM`.
 
-  The arguments a and aM are meant to be `len` limbs in size, i.e. uint32_t[len].
+  The argument a and the outparam aM are meant to be `len` limbs in size, i.e. uint32_t[len].
   The argument k is a montgomery context obtained through Hacl_GenericField32_field_init."]
 val to_field: k:MA.bn_mont_ctx_u32 -> MA.bn_to_field_st k
 
@@ -57,43 +65,43 @@ val to_field: k:MA.bn_mont_ctx_u32 -> MA.bn_to_field_st k
   Write `aM / R mod n` in `a`, i.e.
   Hacl_GenericField32_from_field(k, Hacl_GenericField32_to_field(k, a)) == a % n
 
-  The arguments a and aM are meant to be `len` limbs in size, i.e. uint32_t[len].
+  The argument aM and the outparam a are meant to be `len` limbs in size, i.e. uint32_t[len].
   The argument k is a montgomery context obtained through Hacl_GenericField32_field_init."]
 val from_field: k:MA.bn_mont_ctx_u32 -> MA.bn_from_field_st k
 
 [@@ Comment "Write `aM + bM mod n` in `cM`.
 
-  The arguments aM, bM, and cM are meant to be `len` limbs in size, i.e. uint32_t[len].
+  The arguments aM, bM, and the outparam cM are meant to be `len` limbs in size, i.e. uint32_t[len].
   The argument k is a montgomery context obtained through Hacl_GenericField32_field_init."]
 val add: k:MA.bn_mont_ctx_u32 -> MA.bn_field_add_st k
 
 [@@ Comment "Write `aM - bM mod n` to `cM`.
 
-  The arguments aM, bM, and cM are meant to be `len` limbs in size, i.e. uint32_t[len].
+  The arguments aM, bM, and the outparam cM are meant to be `len` limbs in size, i.e. uint32_t[len].
   The argument k is a montgomery context obtained through Hacl_GenericField32_field_init."]
 val sub: k:MA.bn_mont_ctx_u32 -> MA.bn_field_sub_st k
 
 [@@ Comment "Write `aM * bM mod n` in `cM`.
 
-  The arguments aM, bM, and cM are meant to be `len` limbs in size, i.e. uint32_t[len].
+  The arguments aM, bM, and the outparam cM are meant to be `len` limbs in size, i.e. uint32_t[len].
   The argument k is a montgomery context obtained through Hacl_GenericField32_field_init."]
 val mul: k:MA.bn_mont_ctx_u32 -> MA.bn_field_mul_st k
 
 [@@ Comment "Write `aM * aM mod n` in `cM`.
 
-  The arguments aM and cM are meant to be `len` limbs in size, i.e. uint32_t[len].
+  The argument aM and the outparam cM are meant to be `len` limbs in size, i.e. uint32_t[len].
   The argument k is a montgomery context obtained through Hacl_GenericField32_field_init."]
 val sqr: k:MA.bn_mont_ctx_u32 -> MA.bn_field_sqr_st k
 
 [@@ Comment "Convert a bignum `one` to its Montgomery representation.
 
-  The argument oneM is meant to be `len` limbs in size, i.e. uint32_t[len].
+  The outparam oneM is meant to be `len` limbs in size, i.e. uint32_t[len].
   The argument k is a montgomery context obtained through Hacl_GenericField32_field_init."]
 val one: k:MA.bn_mont_ctx_u32 -> MA.bn_field_one_st k
 
 [@@ Comment "Write `aM ^ b mod n` in `resM`.
 
-  The arguments aM and resM are meant to be `len` limbs in size, i.e. uint32_t[len].
+  The argument aM and the outparam resM are meant to be `len` limbs in size, i.e. uint32_t[len].
   The argument k is a montgomery context obtained through Hacl_GenericField32_field_init.
 
   The argument b is a bignum of any size, and bBits is an upper bound on the
@@ -104,15 +112,15 @@ val one: k:MA.bn_mont_ctx_u32 -> MA.bn_field_one_st k
   This function is constant-time over its argument b, at the cost of a slower
   execution time than exp_vartime.
 
-  Before calling this function, the caller will need to ensure that
-  the following preconditions are observed.
+  Before calling this function, the caller will need to ensure that the following
+  preconditions are observed.
   • 0 < b
   • b < pow2 bBits "]
 val exp_consttime: k:MA.bn_mont_ctx_u32 -> MA.bn_field_exp_consttime_st k
 
 [@@ Comment "Write `aM ^ b mod n` in `resM`.
 
-  The arguments aM and resM are meant to be `len` limbs in size, i.e. uint32_t[len].
+  The argument aM and the outparam resM are meant to be `len` limbs in size, i.e. uint32_t[len].
   The argument k is a montgomery context obtained through Hacl_GenericField32_field_init.
 
   The argument b is a bignum of any size, and bBits is an upper bound on the
@@ -123,19 +131,19 @@ val exp_consttime: k:MA.bn_mont_ctx_u32 -> MA.bn_field_exp_consttime_st k
   The function is *NOT* constant-time on the argument b. See the
   exp_consttime function for constant-time variant.
 
-  Before calling this function, the caller will need to ensure that
-  the following preconditions are observed.
+  Before calling this function, the caller will need to ensure that the following
+  preconditions are observed.
   • 0 < b
   • b < pow2 bBits "]
 val exp_vartime: k:MA.bn_mont_ctx_u32 -> MA.bn_field_exp_vartime_st k
 
 [@@ Comment "Write `aM ^ (-1) mod n` in `aInvM`.
 
-  The arguments aM and aInvM are meant to be `len` limbs in size, i.e. uint32_t[len].
+  The argument aM and the outparam aInvM are meant to be `len` limbs in size, i.e. uint32_t[len].
   The argument k is a montgomery context obtained through Hacl_GenericField32_field_init.
 
-  Before calling this function, the caller will need to ensure that
-  the following preconditions are observed.
+  Before calling this function, the caller will need to ensure that the following
+  preconditions are observed.
   • n is a prime
   • 0 < aM "]
 val inverse: k:MA.bn_mont_ctx_u32 -> MA.bn_field_inv_st k
